Griotte: deep locality and deep immutability (#2)
* WIP add DL and DRO

* WIP add DL and DRO

* WIP add DL and DRO --- FTLR except load

* WIP

* Update logrel for E and sealed to support borrowing + WIP proof FTLR load

* WIP

* Fix V(E,g,---) to include E(RX,g,--) and E(RX,Local,--) + finish proof FTLR

theories/machine_base.v
@@ -13,29 +13,87 @@ From cap_machine Require Export addr_reg solve_addr machine_utils_extra.
 Inductive RXperm : Type :=
 | Orx
 | R
-| X.
+| X
+(* | XSR (* eXecute with System Access Register, high level of execution *) *)
+.
 
 Inductive Wperm : Type :=
 | Ow
 | W
 | WL.
 
+Inductive DLperm : Type :=
+| LG (* Load Global, i.e., does not change the locality bit when loading *)
+| DL (* Deep Local, i.e., any loaded capability set DL and Local *)
+.
+
+Inductive DROperm : Type :=
+| LM (* Load Mutable, i.e., does not change the W permission when loading *)
+| DRO (* Deep RO, i.e., any loaded capability has their Wperm set to Ow *)
+.
+
 Inductive Perm: Type :=
-| BPerm (rx: RXperm) (w: Wperm)
-| E.
+| BPerm (rx: RXperm) (w: Wperm) (dl: DLperm) (dro: DROperm)
+| E     (* Sentry, unseals to (BPerm RX Ow LG LM) *)
+(* | ESR   (* Privileged Sentry, unseals to (BPerm XSR Ow LG LM)  *) *)
+.
 
-Notation O := (BPerm Orx Ow).
+Notation O dl dro := (BPerm Orx Ow dl dro).
 
-Notation WO := (BPerm Orx W).
-Notation WLO := (BPerm Orx WL).
+Notation WO        := (BPerm Orx W LG LM).
+Notation WO_DL     := (BPerm Orx W DL LM).
+Notation WO_DRO    := (BPerm Orx W LG DRO).
+Notation WO_DL_DRO := (BPerm Orx W DL DRO).
 
-Notation RO := (BPerm R Ow).
-Notation RW := (BPerm R W).
-Notation RWL := (BPerm R WL).
+Notation WLO        := (BPerm Orx WL LG LM).
+Notation WLO_DL     := (BPerm Orx WL DL LM).
+Notation WLO_DRO    := (BPerm Orx WL LG DRO).
+Notation WLO_DL_DRO := (BPerm Orx WL DL DRO).
 
-Notation RX := (BPerm X Ow).
-Notation RWX := (BPerm X W).
-Notation RWLX := (BPerm X WL).
+Notation RO        := (BPerm R Ow LG LM).
+Notation RO_DL     := (BPerm R Ow DL LM).
+Notation RO_DRO    := (BPerm R Ow LG DRO).
+Notation RO_DL_DRO := (BPerm R Ow DL DRO).
+
+Notation RW        := (BPerm R W LG LM).
+Notation RW_DL     := (BPerm R W DL LM).
+Notation RW_DRO    := (BPerm R W LG DRO).
+Notation RW_DL_DRO := (BPerm R W DL DRO).
+
+Notation RWL        := (BPerm R WL LG LM).
+Notation RWL_DL     := (BPerm R WL DL LM).
+Notation RWL_DRO    := (BPerm R WL LG DRO).
+Notation RWL_DL_DRO := (BPerm R WL DL DRO).
+
+Notation RX        := (BPerm X Ow LG LM).
+Notation RX_DL     := (BPerm X Ow DL LM).
+Notation RX_DRO    := (BPerm X Ow LG DRO).
+Notation RX_DL_DRO := (BPerm X Ow DL DRO).
+
+Notation RWX        := (BPerm X W LG LM).
+Notation RWX_DL     := (BPerm X W DL LM).
+Notation RWX_DRO    := (BPerm X W LG DRO).
+Notation RWX_DL_DRO := (BPerm X W DL DRO).
+
+Notation RWLX        := (BPerm X WL LG LM).
+Notation RWLX_DL     := (BPerm X WL DL LM).
+Notation RWLX_DRO    := (BPerm X WL LG DRO).
+Notation RWLX_DL_DRO := (BPerm X WL DL DRO).
+
+(* Notation XSR_       := (BPerm XSR Ow LG LM). *)
+(* Notation XSR_DL     := (BPerm XSR Ow DL LM). *)
+(* Notation XSR_DRO    := (BPerm XSR Ow LG DRO). *)
+(* Notation XSR_DL_DRO := (BPerm XSR Ow DL DRO). *)
+
+(* Notation XSRW_       := (BPerm XSR W LG LM). *)
+(* Notation XSRW_DL     := (BPerm XSR W DL LM). *)
+(* Notation XSRW_DRO    := (BPerm XSR W LG DRO). *)
+(* Notation XSRW_DL_DRO := (BPerm XSR W DL DRO). *)
+
+(* Notation XSRWL_       := (BPerm XSR WL LG LM). *)
+(* Notation XSRWL_DL     := (BPerm XSR WL DL LM). *)
+(* Notation XSRWL_DRO    := (BPerm XSR WL LG DRO). *)
+(* Notation XSRWL_DL_DRO := (BPerm XSR WL DL DRO). *)
 
 Inductive Locality: Type :=
 | Global
@@ -101,6 +159,10 @@ Global Instance rxperm_eq_dec : EqDecision RXperm.
 Proof. solve_decision. Defined.
 Global Instance wperm_eq_dec : EqDecision Wperm.
 Proof. solve_decision. Defined.
+Global Instance dlperm_eq_dec : EqDecision DLperm.
+Proof. solve_decision. Defined.
+Global Instance droperm_eq_dec : EqDecision DROperm.
+Proof. solve_decision. Defined.
 Global Instance perm_eq_dec : EqDecision Perm.
 Proof. solve_decision. Defined.
 Global Instance loc_eq_dec : EqDecision Locality.
@@ -122,7 +184,10 @@ Ltac destruct_word w :=
 Ltac destruct_perm p :=
   let rx := fresh "rx" in
   let w := fresh "w" in
-  destruct p as [rx w |]; [destruct rx, w|].
+  let dl := fresh "dl" in
+  let dro := fresh "dro" in
+  (* destruct p as [rx w dl dro | |]; [destruct rx, w, dl, dro| |]. *)
+  destruct p as [rx w dl dro |]; [destruct rx, w, dl, dro|].
 
 Ltac destruct_sealperm p :=
   let b := fresh "b" in
@@ -180,29 +245,45 @@ Definition is_mutable_range (w : Word) : bool:=
   | _ => false end.
 
 (* Auxiliary definitions to work on permissions *)
-(* Definition executeAllowed (p: Perm): bool := *)
-(*   match p with *)
-(*   | RWX | RWLX | RX | E => true *)
-(*   | _ => false *)
-(*   end. *)
+Definition executeAllowed (p: Perm): bool :=
+  match p with
+  | BPerm X _ _ _
+  (* | BPerm XSR _ _ _ *)
+    => true
+  | _ => false
+  end.
 
 Definition readAllowed (p: Perm): bool :=
   match p with
-  | BPerm R _
-  | BPerm X _ => true
+  | BPerm R _ _ _
+  | BPerm X _ _ _
+  (* | BPerm XSR _ _ _ *)
+    => true
   | _ => false
   end.
 
 Definition writeAllowed (p: Perm): bool :=
   match p with
-  | BPerm _ W
-  | BPerm _ WL => true
+  | BPerm _ W _ _
+  | BPerm _ WL _ _=> true
   | _ => false
   end.
 
 Definition pwl p : bool :=
   match p with
-  | BPerm _ WL => true
+  | BPerm _ WL _ _ => true
+  | _ => false
+  end.
+
+Definition isDL p : bool :=
+  match p with
+  | BPerm _ _ DL _ => true
+  | _ => false
+  end.
+
+Definition isDRO p : bool :=
+  match p with
+  | BPerm _ _ _ DRO => true
   | _ => false
   end.
 
@@ -242,6 +323,27 @@ Definition isGlobalWord (w : Word): bool :=
   | WSealable sb => isGlobalSealable sb
   end.
 
+Definition isPerm p p' := @bool_decide _ (perm_eq_dec p p').
+
+Lemma isPerm_refl p : isPerm p p = true.
+Proof. destruct_perm p; auto. Qed.
+Lemma isPerm_ne p p' : p ≠ p' → isPerm p p' = false.
+Proof. intros Hne. destruct_perm p; destruct_perm p'; auto; congruence. Qed.
+
+Definition isPermWord (w : Word) (p : Perm): bool :=
+  match w with
+  | WCap p' _ _ _ _  => isPerm p p'
+  | _ => false
+  end.
+
+Lemma isPermWord_cap_isPerm (w0:Word) p:
+  isPermWord w0 p = true →
+  ∃ p' g b e a, w0 = WCap p' g b e a ∧ isPerm p p' = true.
+Proof.
+  intros Hp. rewrite /isPermWord in Hp.
+  destruct_word w0; try congruence.
+  eexists _, _, _, _, _; split; eauto.
+Qed.
 
 (* Lemma writeA_implies_readA p : *)
 (*   writeAllowed p = true → readAllowed p = true. *)
@@ -276,28 +378,6 @@ Definition writeAllowed_in_r_a (r : Reg) a :=
 
 Definition readAllowed_in_r_a (r : Reg) a :=
   ∃ reg (w : Word), r !! reg = Some w ∧ readAllowedWord w ∧ hasValidAddress w a.
-
-Definition isPerm p p' := @bool_decide _ (perm_eq_dec p p').
-
-Lemma isPerm_refl p : isPerm p p = true.
-Proof. destruct_perm p; auto. Qed.
-Lemma isPerm_ne p p' : p ≠ p' → isPerm p p' = false.
-Proof. intros Hne. destruct_perm p; destruct_perm p'; auto; congruence. Qed.
-
-Definition isPermWord (w : Word) (p : Perm): bool :=
-  match w with
-  | WCap p' _ _ _ _  => isPerm p p'
-  | _ => false
-  end.
-
-Lemma isPermWord_cap_isPerm (w0:Word) p:
-  isPermWord w0 p = true →
-  ∃ p' g b e a, w0 = WCap p' g b e a ∧ isPerm p p' = true.
-Proof.
-  intros Hp. rewrite /isPermWord in Hp.
-  destruct_word w0; try congruence.
-  eexists _, _, _, _, _; split; eauto.
-Qed.
 
 Definition LocalityFlowsTo (l1 l2: Locality): bool :=
   match l1 with
@@ -338,13 +418,21 @@ Definition RXPermFlowsTo (rx1 rx2: RXperm): bool :=
   match rx1 with
   | Orx => true
   | R => match rx2 with
-        | R | X => true
+        | R | X
+        (* | XSR *)
+          => true
         | _ => false
         end
   | X => match rx2 with
-        | X => true
+        | X
+        (* | XSR *)
+          => true
         | _ => false
         end
+  (* | XSR => match rx2 with *)
+  (*       | XSR => true *)
+  (*       | _ => false *)
+  (*       end *)
   end.
 
 Definition WPermFlowsTo (w1 w2 : Wperm) : bool :=
@@ -360,16 +448,38 @@ Definition WPermFlowsTo (w1 w2 : Wperm) : bool :=
          end
   end.
 
+Definition DLPermFlowsTo (dl1 dl2 : DLperm) : bool :=
+  match dl1 with
+  | DL => true
+  | LG => match dl2 with
+             | LG => true
+             | _ => false
+             end
+  end.
+
+Definition DROPermFlowsTo (dro1 dro2 : DROperm) : bool :=
+  match dro1 with
+  | DRO => true
+  | LM => match dro2 with
+             | LM => true
+             | _ => false
+             end
+  end.
 
 Definition PermFlowsTo (p1 p2: Perm): bool :=
   match p1,p2 with
-  | BPerm rx1 w1, BPerm rx2 w2 =>
+  | BPerm rx1 w1 dl1 dro1, BPerm rx2 w2 dl2 dro2 =>
       RXPermFlowsTo rx1 rx2
       && WPermFlowsTo w1 w2
+      && DLPermFlowsTo dl1 dl2
+      && DROPermFlowsTo dro1 dro2
   | E, E => true
-  | E, BPerm rx w =>
+  (* | ESR, ESR => true *)
+  | E, BPerm rx w LG LM =>
       RXPermFlowsTo X rx
-  | BPerm _ _, E => false
+  (* | ESR, BPerm rx w LG LM => *)
+      (* RXPermFlowsTo XSR rx *)
+  | _, _ => false
   end.
 
 Definition PermFlowsToCap (p: Perm) (w: Word) : bool :=
@@ -378,11 +488,98 @@ Definition PermFlowsToCap (p: Perm) (w: Word) : bool :=
   | _ => false
   end.
 
+
+Lemma RXPermFlowsTo_refl : forall rx,  RXPermFlowsTo rx rx.
+Proof.
+  destruct rx; cbn ; done.
+Qed.
+Global Instance RXPermFlowsToReflexive: Reflexive RXPermFlowsTo.
+Proof.
+  rewrite /Reflexive.
+  apply RXPermFlowsTo_refl.
+Qed.
+
+Lemma RXPermFlowsTo_trans : transitive _ RXPermFlowsTo.
+Proof.
+  red; intros.
+  destruct x; destruct y; destruct z; try congruence; auto.
+Qed.
+Global Instance RXPermFlowsToTransitive: Transitive RXPermFlowsTo.
+Proof.
+  rewrite /Transitive.
+  apply RXPermFlowsTo_trans.
+Qed.
+
+Lemma WPermFlowsTo_refl : forall rx,  WPermFlowsTo rx rx.
+Proof.
+  destruct rx; cbn ; done.
+Qed.
+Global Instance WPermFlowsToReflexive: Reflexive WPermFlowsTo.
+Proof.
+  rewrite /Reflexive.
+  apply WPermFlowsTo_refl.
+Qed.
+
+Lemma WPermFlowsTo_trans : transitive _ WPermFlowsTo.
+Proof.
+  red; intros.
+  destruct x; destruct y; destruct z; try congruence; auto.
+Qed.
+Global Instance WPermFlowsToTransitive: Transitive WPermFlowsTo.
+Proof.
+  rewrite /Transitive.
+  apply WPermFlowsTo_trans.
+Qed.
+
+Lemma DLPermFlowsTo_refl : forall rx,  DLPermFlowsTo rx rx.
+Proof.
+  destruct rx; cbn ; done.
+Qed.
+Global Instance DLPermFlowsToReflexive: Reflexive DLPermFlowsTo.
+Proof.
+  rewrite /Reflexive.
+  apply DLPermFlowsTo_refl.
+Qed.
+
+Lemma DLPermFlowsTo_trans : transitive _ DLPermFlowsTo.
+Proof.
+  red; intros.
+  destruct x; destruct y; destruct z; try congruence; auto.
+Qed.
+Global Instance DLPermFlowsToTransitive: Transitive DLPermFlowsTo.
+Proof.
+  rewrite /Transitive.
+  apply DLPermFlowsTo_trans.
+Qed.
+
+Lemma DROPermFlowsTo_refl : forall rx,  DROPermFlowsTo rx rx.
+Proof.
+  destruct rx; cbn ; done.
+Qed.
+Global Instance DROPermFlowsToReflexive: Reflexive DROPermFlowsTo.
+Proof.
+  rewrite /Reflexive.
+  apply DROPermFlowsTo_refl.
+Qed.
+
+Lemma DROPermFlowsTo_trans : transitive _ DROPermFlowsTo.
+Proof.
+  red; intros.
+  destruct x; destruct y; destruct z; try congruence; auto.
+Qed.
+Global Instance DROPermFlowsToTransitive: Transitive DROPermFlowsTo.
+Proof.
+  rewrite /Transitive.
+  apply DROPermFlowsTo_trans.
+Qed.
+
+
 (* Sanity check *)
 Lemma PermFlowsTo_trans:
   transitive _ PermFlowsTo.
 Proof.
-  red; intros; destruct_perm x; destruct_perm y; destruct_perm z; try congruence; auto.
+  red; intros.
+  destruct_perm x; destruct_perm y; destruct_perm z; try congruence; auto.
 Qed.
 
 Global Instance PermFlowsToTransitive: Transitive PermFlowsTo.
@@ -404,6 +601,15 @@ Proof.
   apply PermFlowsTo_refl.
 Qed.
 
+Lemma executeAllowed_flows (p1 p2 : Perm) :
+  PermFlowsTo p1 p2
+  -> executeAllowed p1 = true
+  -> executeAllowed p2 = true.
+Proof.
+  intros Hfl Hxa.
+  destruct_perm p1; destruct_perm p2 ; cbn in *; done.
+Qed.
+
 Lemma readAllowed_flows (p1 p2 : Perm) :
   PermFlowsTo p1 p2
   -> readAllowed p1 = true
@@ -422,69 +628,128 @@ Proof.
   destruct_perm p1; destruct_perm p2 ; cbn in *; done.
 Qed.
 
-Lemma readAllowed_nonO p p' :
-  PermFlowsTo p p' → readAllowed p = true → p' ≠ O.
+Lemma executeAllowed_is_readAllowed (p : Perm) :
+  executeAllowed p = true
+  -> readAllowed p = true.
 Proof.
-  intros Hfl' Hra. destruct_perm p'; auto. destruct_perm p; inversion Hfl'. inversion Hra.
+  intros Hxa.
+  destruct_perm p; cbn in *; done.
 Qed.
 
-Lemma writeAllowed_nonO p p' :
-  PermFlowsTo p p' → writeAllowed p = true → p' ≠ O.
+Lemma notreadAllowed_is_notexecuteAllowed (p : Perm) :
+  readAllowed p = false
+  -> executeAllowed p = false.
 Proof.
-  intros Hfl' Hra. destruct_perm p'; auto. destruct_perm p; inversion Hfl'. inversion Hra.
+  intros Hxa.
+  destruct_perm p; cbn in *; done.
 Qed.
 
-Lemma PCPerm_nonO p p' :
-  PermFlowsTo p p' → p = RX ∨ p = RWX ∨ p = RWLX → p' ≠ O.
+
+Definition isO (p : Perm) : bool :=
+  match p with
+  | BPerm Orx Ow _ _ => true
+  | _ => false
+  end.
+
+Lemma executeAllowed_nonO p p':
+  PermFlowsTo p p' → executeAllowed p = true → isO p' = false.
 Proof.
-  intros Hfl Hvpc. destruct_perm p'; auto. destruct_perm p; inversion Hfl.
-  destruct Hvpc as [Hcontr | [Hcontr | Hcontr]]; inversion Hcontr.
+  intros Hfl' Hxa.
+  eapply executeAllowed_flows in Hxa; eauto.
+  destruct_perm p'; auto; inversion Hxa ; try congruence.
 Qed.
 
-Definition ExecPCPerm p :=
-  p = RX ∨ p = RWX \/ p = RWLX.
-
-Lemma ExecPCPerm_RX: ExecPCPerm RX.
-Proof. left; auto. Qed.
-
-Lemma ExecPCPerm_RWX: ExecPCPerm RWX.
-Proof. right; auto. Qed.
-
-Lemma ExecPCPerm_RWLX: ExecPCPerm RWLX.
-Proof. right; auto. Qed.
-
-Lemma ExecPCPerm_flows_to p p':
-  PermFlowsTo p p' →
-  ExecPCPerm p →
-  ExecPCPerm p'.
+Lemma readAllowed_nonO p p':
+  PermFlowsTo p p' → readAllowed p = true → isO p' = false.
 Proof.
-  intros H [ -> | [ -> | -> ] ]; cbn in H.
-  { destruct_perm p'; cbn in H; try by inversion H; constructor.
-    apply ExecPCPerm_RWX.
-    apply ExecPCPerm_RWLX.
-  }
-  { destruct_perm p'; try by inversion H; constructor.
-    apply ExecPCPerm_RWX.
-    apply ExecPCPerm_RWLX.
-  }
-  { destruct_perm p'; try by inversion H; constructor.
-    apply ExecPCPerm_RWLX.
-  }
+  intros Hfl' Hra.
+  eapply readAllowed_flows in Hra; eauto.
+  destruct_perm p'; auto; inversion Hxa ; try congruence.
 Qed.
 
-Lemma ExecPCPerm_not_E p :
-  ExecPCPerm p →
-  p ≠ E.
+Lemma writeAllowed_nonO p p':
+  PermFlowsTo p p' → writeAllowed p = true → isO p' = false.
 Proof.
-  intros [ H | [H|H] ] ->; inversion H.
+  intros Hfl' Hwa.
+  eapply writeAllowed_flows in Hwa; eauto.
+  destruct_perm p'; auto; inversion Hxa ; try congruence.
 Qed.
 
-Lemma ExecPCPerm_readAllowed p :
-  ExecPCPerm p →
-  readAllowed p = true.
-Proof.
-  intros [ -> | [ -> | -> ] ]; reflexivity.
-Qed.
+(* Definition ExecPCPerm p := *)
+(*   ∃ w dl dro, *)
+(*   p = BPerm X w dl dro \/ p = BPerm XSR w dl dro. *)
+
+(* Lemma X_is_ExecPCPerm p p': *)
+(*    → *)
+(*   ExecPCPerm p → *)
+(*   ExecPCPerm p'. *)
+(* Proof. *)
+(*   intros Hfl Hexec. *)
+(*   destruct Hexec as (w & dl & dro & [Hexec | Hexec] ); subst. *)
+(*   { *)
+(*   destruct_perm p'; cbn in *; try done. *)
+
+
+(* Lemma ExecPCPerm_flows_to p p': *)
+(*   PermFlowsTo p p' → *)
+(*   ExecPCPerm p → *)
+(*   ExecPCPerm p'. *)
+(* Proof. *)
+(*   intros Hfl Hexec. *)
+(*   destruct Hexec as (w & dl & dro & [Hexec | Hexec] ); subst. *)
+(*   { *)
+(*   destruct_perm p'; cbn in *; try done. *)
+
+(*   } *)
+(*   cbn in H. *)
+(*   { destruct_perm p'; cbn in H; try by inversion H; constructor. *)
+(*     apply ExecPCPerm_RWX. *)
+(*     apply ExecPCPerm_RWLX. *)
+(*   } *)
+(*   { destruct_perm p'; try by inversion H; constructor. *)
+(*     apply ExecPCPerm_RWX. *)
+(*     apply ExecPCPerm_RWLX. *)
+(*   } *)
+(*   { destruct_perm p'; try by inversion H; constructor. *)
+(*     apply ExecPCPerm_RWLX. *)
+(*   } *)
+(* Qed. *)
+
+
+(* Lemma PCPerm_nonO p p' dl dro : *)
+(*   PermFlowsTo p p' *)
+(*   → ExecPCPerm p *)
+(*   → p' ≠ (O dl dro). *)
+(* Proof. *)
+(*   intros Hfl Hvpc. *)
+(*   destruct_perm p'; auto. destruct_perm p; inversion Hfl. *)
+(*   destruct Hvpc as [Hcontr | [Hcontr | Hcontr]]; inversion Hcontr. *)
+(* Qed. *)
+
+
+(* Lemma ExecPCPerm_RX: ExecPCPerm RX. *)
+(* Proof. left; auto. Qed. *)
+
+(* Lemma ExecPCPerm_RWX: ExecPCPerm RWX. *)
+(* Proof. right; auto. Qed. *)
+
+(* Lemma ExecPCPerm_RWLX: ExecPCPerm RWLX. *)
+(* Proof. right; auto. Qed. *)
+
+
+(* Lemma ExecPCPerm_not_E p : *)
+(*   ExecPCPerm p → *)
+(*   p ≠ E. *)
+(* Proof. *)
+(*   intros [ H | [H|H] ] ->; inversion H. *)
+(* Qed. *)
+
+(* Lemma ExecPCPerm_readAllowed p : *)
+(*   ExecPCPerm p → *)
+(*   readAllowed p = true. *)
+(* Proof. *)
+(*   intros [ -> | [ -> | -> ] ]; reflexivity. *)
+(* Qed. *)
 
 Definition SealPermFlowsTo (s1 s2 : SealPerms): bool :=
   (if permit_seal(s1) then permit_seal(s2) else true) &&
@@ -526,24 +791,46 @@ Proof.  destruct_sealperm p; destruct_sealperm p'; done. Qed.
 
 (* Helper definitions for capabilities *)
 
-(* Turn E into RX into PC after a jump *)
+(* Turn E into RX, and ESR into XSR after a jump *)
 Definition updatePcPerm (w: Word): Word :=
   match w with
   | WCap E g b e a => WCap RX g b e a
+  (* | WCap ESR g b e a => WCap XSR_ g b e a *)
   | _ => w
   end.
 
 Definition isSentry (p : Perm) : bool :=
  match p with
-   | E => true
-   | BPerm _ _ => false
+   | E
+   (* | ESR *)
+     => true
+   | BPerm _ _ _ _ => false
  end.
 
-Lemma updatePcPerm_cap_non_E p g b e a :
+Lemma executeAllowed_isnot_sentry (p : Perm) :
+  executeAllowed p = true -> isSentry p = false.
+Proof.
+  intros Hexec.
+  destruct_perm p; cbn in *; done.
+Qed.
+
+Definition isE (p : Perm) : bool :=
+ match p with
+   | E => true
+   | _ => false
+ end.
+
+(* Definition isESR (p : Perm) : bool := *)
+(*  match p with *)
+(*    | ESR => true *)
+(*    | _ => false *)
+(*  end. *)
+
+Lemma updatePcPerm_cap_non_sentry p g b e a :
   isSentry p = false ->
   updatePcPerm (WCap p g b e a) = WCap p g b e a.
 Proof.
-  intros HnE. destruct_perm p; cbn in * ; done.
+  intros HnE. destruct_perm p; cbn in *; try done.
 Qed.
 
 Definition nonZero (w: Word): bool :=
@@ -573,7 +860,7 @@ Inductive isCorrectPC: Word → Prop :=
 | isCorrectPC_intro:
     forall p g (b e a : Addr),
       (b <= a < e)%a →
-      p = RX \/ p = RWX \/ p = RWLX →
+      executeAllowed p = true ->
       isCorrectPC (WCap p g b e a).
 
 Lemma isCorrectPC_dec:
@@ -582,63 +869,62 @@ Proof.
   destruct w.
   - right. red; intros H. inversion H.
   - destruct sb as [p g b e a | ].
-    -- case_eq (match p with RX | RWX | RWLX => true | _ => false end); intros.
+    -- case_eq (executeAllowed p); intros.
       + destruct (finz_le_dec b a).
         * destruct (finz_lt_dec a e).
-          { left. econstructor; simpl; eauto. by auto.
-            destruct_perm p; naive_solver. }
+          { left. econstructor; simpl; eauto. by auto. }
           { right. red; intro HH. inversion HH; subst. solve_addr. }
         * right. red; intros HH; inversion HH; subst. solve_addr.
-      + right. red; intros HH; inversion HH; subst. naive_solver.
+      + right. red; intros HH; inversion HH; subst. congruence.
     -- right. red; intros H. inversion H.
  - right. red; intros H. inversion H.
 Qed.
 
-Definition isCorrectPCb (w: Word): bool :=
-  match w with
-  | WCap p g b e a =>
-    (b <=? a)%a && (a <? e)%a &&
-    (isPerm p RX || isPerm p RWX || isPerm p RWLX)
-  | _ => false
-  end.
+(* Definition isCorrectPCb (w: Word): bool := *)
+(*   match w with *)
+(*   | WCap p g b e a => *)
+(*     (b <=? a)%a && (a <? e)%a && *)
+(*     (isPerm p RX || isPerm p RWX || isPerm p RWLX) *)
+(*   | _ => false *)
+(*   end. *)
 
-Lemma isCorrectPCb_isCorrectPC w :
-  isCorrectPCb w = true ↔ isCorrectPC w.
-Proof.
-  rewrite /isCorrectPCb. destruct_word w.
-  1,3,4 : split; try congruence; inversion 1.
-  { rewrite !andb_true_iff !orb_true_iff !Z.leb_le !Z.ltb_lt.
-    rewrite /isPerm !bool_decide_eq_true.
-    split.
-    { intros [? ?]. constructor. solve_addr. naive_solver. }
-    { inversion 1; subst. split. solve_addr. naive_solver. } }
-Qed.
+(* Lemma isCorrectPCb_isCorrectPC w : *)
+(*   isCorrectPCb w = true ↔ isCorrectPC w. *)
+(* Proof. *)
+(*   rewrite /isCorrectPCb. destruct_word w. *)
+(*   1,3,4 : split; try congruence; inversion 1. *)
+(*   { rewrite !andb_true_iff !orb_true_iff !Z.leb_le !Z.ltb_lt. *)
+(*     rewrite /isPerm !bool_decide_eq_true. *)
+(*     split. *)
+(*     { intros [? ?]. constructor. solve_addr. naive_solver. } *)
+(*     { inversion 1; subst. split. solve_addr. naive_solver. } } *)
+(* Qed. *)
 
-Lemma isCorrectPCb_nisCorrectPC w :
-  isCorrectPCb w = false ↔ ¬ isCorrectPC w.
-Proof.
-  destruct (isCorrectPCb w) eqn:HH.
-  { apply isCorrectPCb_isCorrectPC in HH. split; congruence. }
-  { split; auto. intros _. intros ?%isCorrectPCb_isCorrectPC. congruence. }
-Qed.
+(* Lemma isCorrectPCb_nisCorrectPC w : *)
+(*   isCorrectPCb w = false ↔ ¬ isCorrectPC w. *)
+(* Proof. *)
+(*   destruct (isCorrectPCb w) eqn:HH. *)
+(*   { apply isCorrectPCb_isCorrectPC in HH. split; congruence. } *)
+(*   { split; auto. intros _. intros ?%isCorrectPCb_isCorrectPC. congruence. } *)
+(* Qed. *)
 
 Lemma isCorrectPC_ra_wb pc_p pc_g pc_b pc_e pc_a :
   isCorrectPC (WCap pc_p pc_g pc_b pc_e pc_a) →
   readAllowed pc_p && ((pc_b <=? pc_a)%a && (pc_a <? pc_e)%a).
 Proof.
-  intros. inversion H; subst.
-  - destruct H2. apply andb_prop_intro. split.
-    + destruct H6,pc_p; inversion H1; try inversion H2; try inversion H3; auto; try congruence.
+  intros Hcorrect. inversion Hcorrect as [ ? ? ? ? ? Hinbounds Hexec]; subst.
+  - apply executeAllowed_is_readAllowed in Hexec.
+    apply andb_prop_intro; split.
+    + by apply Is_true_eq_left.
     + apply andb_prop_intro.
-      split; apply Is_true_eq_left; [apply Z.leb_le | apply Z.ltb_lt]; lia.
+      split; apply Is_true_eq_left; [apply Z.leb_le | apply Z.ltb_lt]; solve_addr.
 Qed.
 
 Lemma not_isCorrectPC_perm p g b e a :
-  p ≠ RX ∧ p ≠ RWX ∧ p ≠ RWLX → ¬ isCorrectPC (WCap p g b e a).
+  executeAllowed p = false → ¬ isCorrectPC (WCap p g b e a).
 Proof.
-  intros (Hrx & Hrwx & Hrwlx).
-  intros Hvpc. inversion Hvpc;
-    destruct H5 as [Hrx' | [Hrwx' | Hrwlx']]; contradiction.
+  intros Hexec.
+  intros Hvpc; inversion Hvpc; congruence.
 Qed.
 
 Lemma not_isCorrectPC_bounds p g b e a :
@@ -691,9 +977,10 @@ Proof.
 Qed.
 
 Lemma isCorrectPC_nonO p p' g b e a :
-  PermFlowsTo p p' → isCorrectPC (WCap p g b e a) → p' ≠ O.
+  PermFlowsTo p p' → isCorrectPC (WCap p g b e a) → isO p' = false.
 Proof.
-  intros Hfl HcPC. inversion HcPC. by apply (PCPerm_nonO p p').
+  intros Hfl HcPC.
+  inversion HcPC. by apply (executeAllowed_nonO p p').
 Qed.
 
 Lemma isCorrectPC_nonE p g b e a :
@@ -712,12 +999,123 @@ Proof.
   inversion Hvpc; simplify_eq. solve_addr.
 Qed.
 
-Lemma isCorrectPC_ExecPCPerm_InBounds p g b e a :
-  ExecPCPerm p →
+Lemma isCorrectPC_executeAllowed_InBounds p g b e a :
+  executeAllowed p = true →
   InBounds b e a →
   isCorrectPC (WCap p g b e a).
 Proof.
-  unfold ExecPCPerm, InBounds. intros. constructor; eauto.
+  unfold InBounds. intros. constructor; eauto.
+Qed.
+
+
+(* Lemma isCorrectPC_ExecPCPerm_InBounds p g b e a : *)
+(*   ExecPCPerm p → *)
+(*   InBounds b e a → *)
+(*   isCorrectPC (WCap p g b e a). *)
+(* Proof. *)
+(*   unfold ExecPCPerm, InBounds. intros. constructor; eauto. *)
+(* Qed. *)
+
+
+Definition borrow_perm (p : Perm) :=
+  match p with
+  | BPerm rx w _ dro => BPerm rx w DL dro
+  | E => E
+  end.
+
+Definition borrow_sb (sb : Sealable) :=
+  match sb with
+  | SSealRange sp _ b e a => SSealRange sp Local b e a
+  | SCap p _ b e a => SCap (borrow_perm p) Local b e a
+  end.
+
+Definition borrow (w : Word) :=
+  match w with
+  | WSealable sb => WSealable (borrow_sb sb)
+  | WSealed ot sb => WSealed ot (borrow_sb sb)
+  | _ => w
+  end.
+
+Definition readonly_perm (p : Perm) :=
+  match p with
+  | BPerm rx _ dl _ => BPerm rx Ow dl DRO
+  | E => E
+  end.
+
+Definition readonly_sb (sb : Sealable) :=
+  match sb with
+  | SCap p g b e a => SCap (readonly_perm p) g b e a
+  | _ => sb
+  end.
+
+Definition readonly (w : Word) :=
+  match w with
+  | WSealable sb => WSealable (readonly_sb sb)
+  | _ => w
+  end.
+
+Definition load_word (p : Perm) (w : Word) :=
+  let borrow_w := (if isDL p then borrow w else w) in
+  let borrow_dro_w := (if isDRO p then readonly borrow_w else borrow_w) in
+  borrow_dro_w.
+
+Definition load_word_perm (pload p : Perm) :=
+  match p with
+  | BPerm rx pw dl dro => (BPerm rx
+                            (if isDRO pload then Ow else pw)
+                            (if isDL pload then DL else dl)
+                            (if isDRO pload then DRO else dro)
+                         )
+  | E => E
+  end.
+
+Lemma load_word_cap pload p g b e a :
+  load_word pload (WCap p g b e a ) =
+  (WCap (load_word_perm pload p) (if isDL pload then Local else g) b e a).
+Proof.
+  rewrite /load_word /load_word_perm.
+  destruct (isDRO pload) eqn:Hdro,(isDL pload) eqn:Hdl; cbn.
+  all: rewrite /readonly_perm /borrow_perm.
+  all: destruct p; cbn; try done.
+Qed.
+
+Lemma load_word_E (p : Perm) g b e a :
+  load_word p (WCap E g b e a ) = (WCap E (if isDL p then Local else g) b e a ).
+Proof.
+  rewrite /load_word.
+  by destruct (isDRO p),(isDL p); cbn.
+Qed.
+
+Lemma load_word_int p z :
+  load_word p (WInt z) = WInt z.
+Proof.
+  rewrite /load_word.
+  by destruct (isDRO p),(isDL p); cbn.
+Qed.
+
+Lemma load_word_sealrange p sp b g e a :
+  load_word p (WSealRange sp g b e a) = (WSealRange sp (if isDL p then Local else g) b e a).
+Proof.
+  rewrite /load_word.
+  by destruct (isDRO p),(isDL p); cbn.
+Qed.
+
+Lemma load_word_sealed p ot sb  :
+  load_word p (WSealed ot sb) = (WSealed ot (if isDL p then borrow_sb sb else sb)).
+Proof.
+  rewrite /load_word /borrow_sb.
+  destruct (isDRO p) eqn:Hdro,(isDL p) eqn:Hdl; cbn; auto.
+Qed.
+
+Lemma load_word_perm_flows (pload p : Perm) :
+  PermFlowsTo (load_word_perm pload p) p.
+Proof.
+  destruct p; last done.
+  repeat (apply andb_True;split).
+  + reflexivity.
+  + destruct (isDRO pload) eqn:Hdro; done.
+  + destruct (isDL pload) eqn:Hdl; done.
+  + destruct (isDRO pload) eqn:Hdro; done.
 Qed.
 
 (* Useful instances *)
@@ -729,12 +1127,14 @@ Proof.
           | Orx => 1
           | R => 2
           | X => 3
+          (* | XSR => 4 *)
           end%positive.
   set decode :=
     fun n => match n with
     | 1 => Some Orx
     | 2 => Some R
     | 3 => Some X
+    (* | 4 => Some XSR *)
     | _ => None
     end%positive.
   eapply (Build_Countable _ _ encode decode).
@@ -760,17 +1160,53 @@ Proof.
   intro p. destruct p; reflexivity.
 Defined.
 
+Global Instance dlperm_countable : Countable DLperm.
+Proof.
+  set encode :=
+    fun p => match p with
+          | DL => 1
+          | LG => 2
+          end%positive.
+  set decode :=
+    fun n => match n with
+    | 1 => Some DL
+    | 2 => Some LG
+    | _ => None
+    end%positive.
+  eapply (Build_Countable _ _ encode decode).
+  intro p. destruct p; reflexivity.
+Defined.
+
+Global Instance droperm_countable : Countable DROperm.
+Proof.
+  set encode :=
+    fun p => match p with
+          | DRO => 1
+          | LM => 2
+          end%positive.
+  set decode :=
+    fun n => match n with
+    | 1 => Some DRO
+    | 2 => Some LM
+    | _ => None
+    end%positive.
+  eapply (Build_Countable _ _ encode decode).
+  intro p. destruct p; reflexivity.
+Defined.
+
 Global Instance perm_countable : Countable Perm.
 Proof.
   set encode :=
     fun p => match p with
-          | BPerm rx w => inl (rx,w)
+          | BPerm rx w dl dro=> inl (rx,w,dl,dro)
           | E => inr ()
+          (* | ESR => inr false *)
           end.
   set decode :=
     fun n => match n with
-          | inl (rx,w) => BPerm rx w
+          | inl (rx,w,dl,dro) => BPerm rx w dl dro
           | inr () => E
+          (* | inr false => ESR *)
           end.
   refine (inj_countable' encode decode _).
   intro p. destruct p; reflexivity.
@@ -931,8 +1367,130 @@ Qed.
 Global Instance readAllowed_in_r_a_Decidable r a: Decision (readAllowed_in_r_a r a).
 Proof.
   eapply finite.exists_dec.
-  intros x. destruct (r !! x) eqn:Hsome;
+  intros x.
+  destruct (r !! x) eqn:Hsome;
     first destruct (decide (readAllowedWord w)), (decide (hasValidAddress w a)).
-  left. eexists _; auto.
+  left. eexists _; eauto.
   all : (right; intros [w1 (Heq & ? & ?)]; inversion Heq; try congruence ).
+Qed.
+
+
+(* TODO re organise *)
+Lemma readAllowed_isnot_sentry (p : Perm) :
+  readAllowed p = true -> isSentry p = false.
+Proof.
+  intros Hexec.
+  destruct_perm p; cbn in *; done.
+Qed.
+
+Lemma writeAllowed_isnot_sentry (p : Perm) :
+  writeAllowed p = true -> isSentry p = false.
+Proof.
+  intros Hexec.
+  destruct_perm p; cbn in *; done.
+Qed.
+
+Lemma pwl_flows (p1 p2 : Perm) :
+  PermFlowsTo p1 p2
+  -> pwl p1 = true
+  -> pwl p2 = true.
+Proof.
+  intros Hfl Hra.
+  destruct_perm p1; destruct_perm p2 ; cbn in *; done.
+Qed.
+
+Lemma pwl_nonO p p':
+  PermFlowsTo p p' → pwl p = true → isO p' = false.
+Proof.
+  intros Hfl' Hra.
+  eapply pwl_flows in Hra; eauto.
+  destruct_perm p'; auto; inversion Hxa ; try congruence.
+Qed.
+
+Lemma pwl_isnot_sentry (p : Perm) :
+  pwl p = true -> isSentry p = false.
+Proof.
+  intros Hexec.
+  destruct_perm p; cbn in *; done.
+Qed.
+
+Lemma isnotO_flows (p p' : Perm) :
+  PermFlowsTo p p'
+  -> isO p' = true
+  -> isO p = true.
+Proof.
+  intros Hfl Hra.
+  destruct_perm p; destruct_perm p' ; cbn in *; done.
+Qed.
+
+Lemma isO_flows (p p' : Perm) :
+  PermFlowsTo p p'
+  -> isO p = false
+  -> isO p' = false.
+Proof.
+  intros Hfl Hra.
+  destruct_perm p; destruct_perm p' ; cbn in *; done.
+Qed.
+
+Lemma isDRO_flows (p p' : Perm) :
+  PermFlowsTo p p' ->
+  isDRO p' = true ->
+  isDRO p = true.
+Proof.
+  intros Hfl Hra.
+  destruct_perm p; destruct_perm p' ; cbn in *; done.
+Qed.
+
+Lemma isDL_flows (p p' : Perm) :
+  PermFlowsTo p p' ->
+  isDL p' = true ->
+  isDL p = true.
+Proof.
+  intros Hfl Hra.
+  destruct_perm p; destruct_perm p' ; cbn in *; done.
+Qed.
+
+Lemma isnotDRO_flows (p p' : Perm) :
+  PermFlowsTo p p' ->
+  isDRO p = false ->
+  isDRO p' = false.
+Proof.
+  intros Hfl Hra.
+  destruct_perm p; destruct_perm p' ; cbn in *; done.
+Qed.
+
+Lemma isnotDL_flows (p p' : Perm) :
+  PermFlowsTo p p' ->
+  isDL p = false ->
+  isDL p' = false.
+Proof.
+  intros Hfl Hra.
+  destruct_perm p; destruct_perm p' ; cbn in *; done.
+Qed.
+
+Lemma load_word_perm_load_flows (pload pload' p : Perm) :
+  PermFlowsTo pload pload' ->
+  PermFlowsTo (load_word_perm pload p) (load_word_perm pload' p).
+Proof.
+  intro Hfl.
+  destruct p; cbn; last done.
+  repeat (apply andb_True;split).
+  + reflexivity.
+  + destruct (isDRO pload) eqn:Hdro; first done.
+    apply isnotDRO_flows in Hfl; auto.
+    by rewrite Hfl.
+  + destruct (isDL pload) eqn:Hdl; first done.
+    apply isnotDL_flows in Hfl; auto.
+    by rewrite Hfl.
+  + destruct (isDRO pload) eqn:Hdro; first done.
+    apply isnotDRO_flows in Hfl; auto.
+    by rewrite Hfl.
+Qed.
+
+Lemma isO_load_word (pload p : Perm) :
+  isO p = true -> isO (load_word_perm pload p) = true.
+Proof.
+  intros HO.
+  destruct_perm p; cbn in * ; try congruence.
+  all: by rewrite Tauto.if_same.
 Qed.
