theories/ftlr/interp_weakening.v
@@ -1,9 +1,8 @@
-From cap_machine Require Export logrel.
 From iris.proofmode Require Import proofmode.
 From iris.program_logic Require Import weakestpre adequacy lifting.
 From stdpp Require Import base.
-From cap_machine.ftlr Require Import ftlr_base.
 From cap_machine Require Import addr_reg region monotone.
+From cap_machine Require Export logrel ftlr_base.
 
 Section fundamental.
   Context
@@ -25,11 +24,38 @@ Section fundamental.
   Implicit Types w : (leibnizO Word).
   Implicit Types interp : (D).
 
+  Lemma interp_weakening_from_E W g b e a :
+      interp W (WCap E g b e a)
+      -∗ interp W (WCap E Local b e a).
+  Proof.
+    iIntros "#Hinterp".
+    rewrite !fixpoint_interp1_eq !interp1_eq.
+    replace (isO E) with false ; auto.
+    replace (isSentry E) with true ; auto.
+    iDestruct "Hinterp" as "#Hinterp".
+    iModIntro.
+    rewrite /enter_cond /interp_expr /=.
+    iIntros (regs W' Hrelated).
+    destruct g.
+    - iAssert (future_world Global W W')%I as "%Hrelated'".
+      { iPureIntro.
+        apply related_sts_pub_priv_trans_world with W', related_sts_priv_refl_world; auto.
+      }
+      iSpecialize ("Hinterp" $! regs W' Hrelated').
+      iDestruct "Hinterp" as "[Hinterp Hinterp_borrowed]".
+      iSplitL; iFrame "#".
+    - iAssert (future_world Local W W')%I as "%Hrelated'".
+      { done. }
+      iSpecialize ("Hinterp" $! regs W' Hrelated').
+      iDestruct "Hinterp" as "[Hinterp Hinterp_borrowed]".
+      iSplitL; iFrame "#".
+  Qed.
+
   Lemma interp_weakeningEO W p p' g g' b b' e e' a a' :
     isSentry p = false ->
-    p ≠ O →
+    isO p = false →
     isSentry p' = false ->
-    p' ≠ O →
+    isO p' = false →
     (b <= b')%a ->
     (e' <= e)%a ->
     PermFlowsTo p' p ->
@@ -39,9 +65,7 @@ Section fundamental.
   Proof.
     intros HpnotE HpnotO HpnotE' HpnotO' Hb He Hp Hl. iIntros "HA".
     rewrite !fixpoint_interp1_eq !interp1_eq.
-    destruct (decide (p = O)) as [|_];try congruence.
-    destruct (decide (p' = O)) as [|_];try congruence.
-    rewrite HpnotE HpnotE'.
+    rewrite HpnotO HpnotO' HpnotE HpnotE'.
     iDestruct "HA" as "[#A %Hpwl_cond]".
     iSplit; cycle 1.
     { case_eq (pwl p'); intros Hpwl'; auto.
@@ -98,7 +122,7 @@ Section fundamental.
 
   Lemma interp_weakeningE W p g g' b b' e e' a a' :
       isSentry p = false ->
-      p <> O ->
+      isO p = false ->
       (b <= b')%a ->
       (e' <= e)%a ->
       PermFlowsTo E p ->
@@ -110,26 +134,32 @@ Section fundamental.
     intros HpnotE HpnotO Hb He Hp Hl.
     iIntros "#IH HA".
     rewrite !fixpoint_interp1_eq !interp1_eq.
-    destruct (decide (p = O)) as [|_];try congruence.
-    rewrite HpnotE.
-    erewrite decide_False;auto; cbn.
+    rewrite HpnotO HpnotE.
+    replace (isO E) with false ; auto.
+    replace (isSentry E) with true ; auto.
     iDestruct "HA" as "[#A %Hpwl_cond]".
     iModIntro.
     rewrite /enter_cond /interp_expr /=.
-    iIntros (r W') "#Hfuture". iNext.
-    iIntros "[[Hfull Hmap] [Hreg [Hregion [Hsts Hown]]]]".
-    rewrite /interp_conf.
-    iApply ("IH" with "Hfull Hmap Hreg Hregion Hsts Hown"); eauto.
-    iModIntro. rewrite fixpoint_interp1_eq /=.
-    simpl. destruct (decide (b' < e'))%a.
-    - rewrite (isWithin_finz_seq_between_decomposition b' e' b e); try solve_addr.
+    iIntros (r W') "#Hfuture".
+    iSplitR; iNext.
+    - iIntros "[[Hfull Hmap] [Hreg [Hregion [Hsts Hown]]]]".
+      rewrite /interp_conf.
+      iApply ("IH" with "Hfull Hmap Hreg Hregion Hsts Hown"); eauto.
+      iModIntro. rewrite fixpoint_interp1_eq /=.
+      destruct (decide (b' < e'))%a; cycle 1.
+      { rewrite (finz_seq_between_empty b' e'); auto; solve_addr. }
+      rewrite (isWithin_finz_seq_between_decomposition b' e' b e); try solve_addr.
       rewrite !big_sepL_app. iDestruct "A" as "[_ [A2 _]]".
       iApply (big_sepL_impl with "A2"); auto.
       iModIntro; iIntros (k x Hx) "Hw".
       iDestruct "Hw" as (p'' φ Hflp'' Hpersφ) "(Hrel & #Hzcond & #Hrcond & #Hwcond & #HmonoR & %Hstate)".
       assert (Hflows': PermFlowsTo RX p'').
       { eapply PermFlowsTo_trans; eauto.
-        destruct p; simpl in *; auto; try congruence; try tauto; reflexivity. }
+        destruct p; cbn in HpnotE ; try done.
+        destruct dl; cbn in Hp; try done.
+        destruct dro; cbn in Hp; try done.
+        destruct rx; cbn in Hp; try done.
+      }
       iExists p'',φ.
       replace (readAllowed p) with true; cycle 1.
       { destruct_perm p ; cbn in *; try done. }
@@ -138,7 +168,62 @@ Section fundamental.
                   with "[$Hfuture] [] [$HmonoR]") as "HmonoR'"; eauto.
       repeat(iSplit; auto).
       iApply (region_state_nwl_future with "Hfuture"); eauto.
-    - rewrite (finz_seq_between_empty b' e'); auto; solve_addr.
+
+    - iIntros "[[Hfull Hmap] [Hreg [Hregion [Hsts Hown]]]]".
+      rewrite /interp_conf.
+      iApply ("IH" with "Hfull Hmap Hreg Hregion Hsts Hown"); eauto.
+      iModIntro. rewrite fixpoint_interp1_eq /=.
+      destruct (decide (b' < e'))%a; cycle 1.
+      { rewrite (finz_seq_between_empty b' e'); auto; solve_addr. }
+      rewrite (isWithin_finz_seq_between_decomposition b' e' b e); try solve_addr.
+      rewrite !big_sepL_app. iDestruct "A" as "[_ [A2 _]]".
+      iApply (big_sepL_impl with "A2"); auto.
+      iModIntro; iIntros (k x Hx) "Hw".
+      iDestruct "Hw" as (p'' φ Hflp'' Hpersφ) "(Hrel & #Hzcond & #Hrcond & #Hwcond & #HmonoR & %Hstate)".
+      assert (Hflows': PermFlowsTo RX p'').
+      { eapply PermFlowsTo_trans; eauto.
+        destruct p; cbn in HpnotE ; try done.
+        destruct dl; cbn in Hp; try done.
+        destruct dro; cbn in Hp; try done.
+        destruct rx; cbn in Hp; try done.
+      }
+      iExists p'',φ.
+      replace (readAllowed p) with true; cycle 1.
+      { destruct_perm p ; cbn in *; try done. }
+      iFrame "Hrel".
+
+      destruct (pwl p) eqn: Hpwl; cycle 1.
+      { assert (if pwl p then g = Local else True) as Hpwl_cond' by (rewrite Hpwl //=).
+        assert (
+           if pwl p then region_state_pwl W x else region_state_nwl W x g
+          ) as Hstate' by (rewrite Hpwl //=).
+       iDestruct ( (monoReq_nwl_future W W' g g' p p'' x φ)
+                  with "[$Hfuture] [] [$HmonoR]") as "HmonoR'"; eauto.
+       repeat(iSplit; auto).
+       iDestruct (region_state_nwl_future with "Hfuture") as "Hregion_state" ; eauto.
+       iSpecialize ("Hregion_state" $! Hstate').
+       destruct g'; cbn; [iLeft|]; done.
+      }
+      { assert (if pwl p then g = Local else True) as Hpwl_cond' by (rewrite Hpwl //=).
+        assert (
+           if pwl p then region_state_pwl W x else region_state_nwl W x g
+          ) as Hstate' by (rewrite Hpwl //=).
+        repeat(iSplit; auto).
+
+        destruct g'; cbn.
+        { (* contradiction *)
+          destruct g; first congruence; done.
+        }
+        iDestruct "Hfuture" as "%Hfuture".
+        iApply monoReq_mono_pub_pwl; eauto.
+
+        destruct g'; cbn.
+        { (* contradiction *)
+          destruct g; first congruence; done.
+        }
+        iDestruct "Hfuture" as "%Hfuture".
+        eapply region_state_pwl_monotone in Hstate; eauto.
+      }
   Qed.
 
   Lemma interp_weakening W p p' g g' b b' e e' a a' :
@@ -152,24 +237,27 @@ Section fundamental.
     interp W (WCap p' g' b' e' a').
   Proof.
     intros HpnotE Hb He Hp Hl. iIntros "#IH HA".
-    destruct (decide (p' = O)).
-    { subst; rewrite !fixpoint_interp1_eq !interp1_eq; auto. }
-    destruct (decide (p = O)).
-    { subst p; destruct_perm p'; simpl in Hp; try tauto. }
+    destruct (isO p') eqn:HpO'.
+    { rewrite !fixpoint_interp1_eq !interp1_eq HpO'; auto. }
+    destruct (isO p) eqn:HpO.
+    { eapply isnotO_flows in Hp ; eauto; congruence. }
     destruct (isSentry p') eqn:Hsentryp'; cycle 1.
     { iApply (interp_weakeningEO _ p p' g g'); eauto. }
-    { destruct p, p' ; cbn in * ; try congruence. iApply (interp_weakeningE _ (BPerm rx w) g g'); eauto. }
+    { destruct p, p' ; cbn in * ; try congruence.
+      iApply (interp_weakeningE _ (BPerm rx w dl dro) g g'); eauto.
+    }
   Qed.
 
   Lemma interp_next_PC W p g b e a a' :
     isCorrectPC (WCap p g b e a) ->
-    ftlr_IH -∗
     interp W (WCap p g b e a) -∗
     interp W (WCap p g b e a').
   Proof.
-    iIntros (HcorrectPC) "#IH #Hinterp".
-    iApply interp_weakening; eauto; try solve_addr; try done.
-    by eapply isCorrectPC_nonE.
+    iIntros (HcorrectPC) "#Hinterp".
+    inversion HcorrectPC as [p' g' b' e' a'' Hb' Hexec']; subst.
+    assert (isO p = false) by (by eapply executeAllowed_nonO).
+    assert (isSentry p = false) by (by eapply executeAllowed_isnot_sentry).
+    iApply interp_weakeningEO; eauto; try solve_addr; try done.
   Qed.
 
   Lemma safe_to_unseal_weakening b e b' e':
@@ -214,6 +302,174 @@ Section fundamental.
   all: destruct (permit_unseal p') eqn:Hunseal; [eapply (permit_unseal_flowsto _ p) in Hunseal as ->; auto | ]; iDestruct "HA" as "[Hs Hus]".
   all: iSplitL "Hs";
   [try iApply (safe_to_seal_weakening with "Hs") | try iApply (safe_to_unseal_weakening with "Hus")]; auto.
+  Qed.
+
+  Lemma interp_borrowed_sealed (W : WORLD) (ot : OType) (sb : Sealable) :
+    interp W (WSealed ot sb) -∗ interp W (WSealed ot (borrow_sb sb)).
+  Proof.
+    iIntros "Hinterp".
+    rewrite !fixpoint_interp1_eq /= /interp_sb.
+    iDestruct "Hinterp" as (P HpersP) "(Hsealpred & _ & HPborrowed)".
+    iDestruct "HPborrowed" as "#HPborrowed".
+    replace (borrow (WSealable (borrow_sb sb)))
+      with (WSealable (borrow_sb sb)).
+    iFrame "∗#%".
+    cbn.
+    destruct sb; auto.
+    destruct p; auto.
+  Qed.
+
+  Lemma interp_load_word W p w : interp W w ⊢ interp W (load_word p w).
+  Proof.
+    iIntros "Hinterp".
+    destruct w.
+    - by rewrite load_word_int.
+    - destruct sb; try done; cbn; cycle 1.
+      { rewrite load_word_sealrange.
+        by rewrite !fixpoint_interp1_eq.
+      }
+      {
+        destruct p0; [ rewrite load_word_cap | rewrite load_word_E ];cycle 1.
+        { destruct (isDL p); last done.
+          by iApply interp_weakening_from_E.
+        }
+        rewrite !fixpoint_interp1_eq !interp1_eq.
+
+        destruct (isO (BPerm rx w dl dro)) eqn:HpO.
+        { destruct rx,w; cbn in *; try done.
+          by rewrite Tauto.if_same.
+        }
+        set (w' := (if isDRO p then Ow else w)).
+        set (dl' := (if isDL p then DL else dl)).
+        set (dro' := (if isDRO p then DRO else dro)).
+        destruct (isO (load_word_perm p (BPerm rx w dl dro))); first done.
+        replace (isSentry (BPerm rx w dl dro)) with false; auto.
+        replace (isSentry (load_word_perm p (BPerm rx w dl dro))) with false; auto.
+
+        iDestruct "Hinterp" as "[Hinterp %Hw]".
+        iSplit; cycle 1.
+        iPureIntro.
+        {
+          rewrite /load_word_perm.
+          destruct (isDRO p); subst w'; cbn; try done.
+          destruct w; try done.
+          cbn in Hw.
+          subst; by rewrite Tauto.if_same.
+        }
+        iApply (big_sepL_mono with "Hinterp").
+        iIntros (k y Hky) "Ha".
+        iDestruct "Ha" as
+          (p' P' Hflp' HpersP')
+            "(Hrel & Hzcond & Hrcond & Hwcond & HmonoR & %Hstate)".
+        iExists p',P'.
+        iFrame "∗".
+        iSplit;[iPureIntro|].
+        {
+          transitivity (BPerm rx w dl dro); auto.
+          apply load_word_perm_flows.
+        }
+        iSplit;[iFrame "%"|].
+        iPureIntro.
+        destruct (pwl (BPerm rx w dl dro)) eqn:Hpwl ; simplify_eq.
+        { rewrite /load_word_perm.
+          cbn in Hpwl; destruct w ; try congruence.
+          destruct (isDRO p); subst w'; cbn; auto.
+          rewrite Tauto.if_same; cbn.
+          by right.
+        }
+        { assert (pwl (load_word_perm p (BPerm rx w dl dro)) = false) as ->.
+          { cbn in *.
+            subst w'.
+            destruct (isDRO p); done.
+          }
+          destruct (isDL p); cbn; auto.
+          destruct g; cbn in Hstate; naive_solver.
+        }
+      }
+    - rewrite load_word_sealed.
+      destruct (isDL p); auto.
+      by iApply (interp_borrowed_sealed with "Hinterp").
+  Qed.
+
+  Lemma interp_borrow_word W w : interp W w ⊢ interp W (borrow w).
+  Proof.
+    iIntros "Hw".
+    iDestruct (interp_load_word W RO_DL w with "Hw") as "Hw'".
+    by cbn.
+  Qed.
+
+  Lemma interp_readonly_word W w : interp W w ⊢ interp W (readonly w).
+  Proof.
+    iIntros "Hw".
+    iDestruct (interp_load_word W RO_DRO w with "Hw") as "Hw'".
+    by cbn.
+  Qed.
+
+  Lemma interp_weakening_word_load (W : WORLD) (p p' : Perm) v :
+    PermFlowsTo p p'
+    -> fixpoint interp1 W (load_word p' v)
+    -∗ fixpoint interp1 W (load_word p v).
+  Proof.
+    iIntros (Hfl) "#Hinterp".
+    destruct v.
+    - rewrite !load_word_int; done.
+    - destruct sb; cycle 1.
+      { rewrite !load_word_sealrange; cbn.
+        by rewrite !fixpoint_interp1_eq /=.
+      }
+      destruct p0 as [ rx0 w0 dl0 dro0|]; cycle 1.
+      { rewrite !load_word_E.
+        destruct (isDL p') eqn:Hdl
+        ; [ eapply isDL_flows in Hfl; eauto ; rewrite Hfl |]
+        ; auto.
+        destruct (isDL p); auto.
+        by iApply interp_weakening_from_E.
+      }
+      rewrite !load_word_cap.
+      destruct (isO (load_word_perm p (BPerm rx0 w0 dl0 dro0))) eqn:HnO.
+      { rewrite !fixpoint_interp1_eq !interp1_eq.
+        by rewrite HnO.
+      }
+      destruct (isSentry (BPerm rx0 w0 dl0 dro0)) eqn:Hnsentry.
+      { cbn in Hnsentry ; congruence . }
+      iApply (interp_weakeningEO with "Hinterp"); auto; try solve_addr.
+      + eapply isO_flows ; eauto.
+        apply load_word_perm_load_flows;auto.
+      + apply load_word_perm_load_flows;auto.
+      + destruct (isDL p) eqn:Hdl; auto.
+        eapply isnotDL_flows in Hfl; eauto.
+        by rewrite Hfl.
+    - rewrite !load_word_sealed.
+      destruct (isDL p') eqn:Hdl'; cbn.
+      + pose proof (isDL_flows p p' Hfl Hdl') as Hdl; rewrite Hdl.
+        done.
+      + iDestruct (interp_borrowed_sealed with "Hinterp") as "Hinterp'".
+        destruct (isDL p); auto.
+  Qed.
+
+  (* Lemmas about interp  *)
+
+  Lemma interp_int W n : ⊢ interp W (WInt n).
+  Proof. iIntros. rewrite /interp fixpoint_interp1_eq //. Qed.
+
+  Lemma persistent_cond_interp : persistent_cond interp.
+  Proof.
+    intros W; apply _.
+  Qed.
+  Lemma zcond_interp : ⊢ zcond interp.
+  Proof.
+    by iModIntro; iIntros (W1 W2 w) "_"; iApply interp_int.
+  Qed.
+
+  Lemma wcond_interp : ⊢ wcond interp interp.
+  Proof.
+    by iModIntro; iIntros (W1 w) "?".
+  Qed.
+
+  Lemma rcond_interp p : ⊢ rcond p interp interp.
+  Proof.
+    iModIntro; iIntros (W1 w) "?".
+    by iApply interp_load_word.
   Qed.
 
 End fundamental.
